Lean4Lean/Verify/Typing/EnvLemmas.lean
@@ -17,8 +17,6 @@ theorem TrDefVal.mono {env env' : VEnv} (henv : env ≤ env')
     (H : TrDefVal safety env ci ci') : TrDefVal safety env' ci ci' :=
   ⟨H.1.mono henv, H.2.mono henv⟩
 
-section
-
 variable (safety : DefinitionSafety) (env : VEnv) in
 inductive Aligned1 : ConstantInfo → Option VConstant → Prop where
   | block : ¬isAsSafeAs safety ci → Aligned1 ci none
@@ -28,14 +26,14 @@ variable (safety : DefinitionSafety) in
 inductive Aligned : ConstMap → VEnv → Prop where
   | empty : Aligned {} .empty
   | const : Aligned C venv → Aligned1 safety venv ci ci' →
-    venv.addConst n ci' = some venv' → Aligned (C.insert n ci) venv'
+    venv.addConst n ci' = some venv' → ci.name = n → Aligned (C.insert n ci) venv'
   | defeq : Aligned C venv → Aligned C (venv.addDefEq df)
 
 theorem Aligned.map_wf' (H : Aligned safety C venv) :
     C.WF ∧ ∀ n, (C.find? n).isSome = (venv.constants n).isSome := by
   induction H with
   | empty => exact ⟨.empty, by simp [SMap.find?, VEnv.empty]⟩
-  | @const _ _ _ _ n _ _ _ eq ih =>
+  | @const _ _ _ _ n _ _ _ eq _ ih =>
     simp [VEnv.addConst] at eq; split at eq <;> cases eq
     have := ih.2 n; simp_all [-ih]
     refine ⟨.insert ih.1 _ _ this, fun n' => ?_⟩
@@ -50,7 +48,7 @@ theorem Aligned.addQuot1 {Q : Prop}
     (H1 : ∀ c env, Aligned safety c env → P c env → Q)
     (C env) (wf : Aligned safety C env) (H2 : AddQuot1 n k ci P C env) : Q := by
   let ⟨_, _, h1, h2, h3, h4⟩ := H2
-  refine H1 _ _ (wf.const (.const ⟨by cases safety <;> rfl, h2.2⟩) h3) h4
+  exact H1 _ _ (wf.const (.const ⟨by cases safety <;> rfl, h2.2⟩) h3 rfl) h4
 
 nonrec theorem Aligned.addQuot (H : AddQuot C₁ C₂ venv₁ venv₂)
     (wf : Aligned safety C₁ venv₁) : Aligned safety C₂ venv₂ := by
@@ -65,10 +63,10 @@ theorem Aligned.addInduct (H : AddInduct C₁ venv₁ decl C₂ venv₂) :
 theorem TrEnv'.aligned (H : TrEnv' safety C Q venv) : Aligned safety C venv := by
   induction H with
   | empty => exact .empty
-  | block hs h _ ih => exact ih.const (.block hs) h
-  | «axiom» h1 _ h _ ih => exact ih.const (.const h1) h
-  | «opaque» h1 _ h _ ih => exact ih.const (.const h1.1.1) h
-  | defn h1 _ h _ ih => exact (ih.const (.const h1.1.1) h).defeq
+  | block hs h _ ih => exact ih.const (.block hs) h rfl
+  | «axiom» h1 _ h _ ih => exact ih.const (.const h1) h rfl
+  | «opaque» h1 _ h _ ih => exact ih.const (.const h1.1.1) h rfl
+  | defn h1 _ h _ ih => exact (ih.const (.const h1.1.1) h rfl).defeq
   | quot _ h _ ih => exact ih.addQuot h
   | induct _ h _ ih => exact ih.addInduct h
 
@@ -83,10 +81,10 @@ theorem Aligned.find? (H : Aligned safety C venv)
     | ⟨_, h1, h2⟩ => ⟨_, H.constants h1, h2.mono H⟩
   induction H with
   | empty => simp [SMap.find?] at h
-  | const h1 h2 h3 ih =>
+  | const h1 h2 h3 h4 ih =>
     have := VEnv.addConst_le h3
     rw [h1.map_wf.find?_insert] at h; split at h
-    · cases h; rename_i n _ h; simp at h; subst n
+    · cases h; rename_i n _ h; simp at h; subst n h
       simp [VEnv.addConst] at h3; split at h3 <;> cases h3
       cases h2; · contradiction
       simp; rename_i h'; exact h'.mono this
@@ -95,19 +93,17 @@ theorem Aligned.find? (H : Aligned safety C venv)
 
 theorem Aligned.find?_uniq (H : Aligned safety C venv)
     (h : C.find? name = some ci) (hs : venv.constants name = some (some ci')) :
-    TrConstant safety venv ci ci' := by
+    ci.name = name ∧ TrConstant safety venv ci ci' := by
   induction H with
   | empty => simp [SMap.find?] at h
-  | const h1 h2 h3 ih =>
+  | const h1 h2 h3 h4 ih =>
     have := VEnv.addConst_le h3
     simp [VEnv.addConst] at h3; split at h3 <;> cases h3
     simp [h1.map_wf.find?_insert] at h hs; revert h hs; split
     · rintro ⟨⟩ ⟨⟩; rename_i n _ _ _; subst n
-      let .const h2 := h2; exact h2.mono this
-    · intro hs h; exact (ih h hs).mono this
-  | defeq h1 ih => exact (ih h hs).mono VEnv.addDefEq_le
-
-end
+      let .const h2 := h2; exact ⟨h4, h2.mono this⟩
+    · intro hs h; let ⟨h1, h2⟩ := ih h hs; exact ⟨h1, h2.mono this⟩
+  | defeq h1 ih => let ⟨h1, h2⟩ := ih h hs; exact ⟨h1, h2.mono VEnv.addDefEq_le⟩
 
 theorem TrEnv.find?_iff (H : TrEnv safety env venv) :
     (∃ ci, env.find? name = some ci) ↔ ∃ oci, venv.constants name = some oci := by
@@ -121,5 +117,44 @@ theorem TrEnv.find? (H : TrEnv safety env venv)
 
 theorem TrEnv.find?_uniq (H : TrEnv safety env venv)
     (h : env.find? name = some ci) (hs : venv.constants name = some (some ci')) :
-    TrConstant safety venv ci ci' :=
+    ci.name = name ∧ TrConstant safety venv ci ci' :=
   H.aligned.find?_uniq (H.map_wf.find?'_eq_find? _ ▸ h) hs
+
+theorem TrEnv'.of_value (H : TrEnv' safety C Q venv) (h : C.find? name = some ci)
+    (hs : isAsSafeAs safety ci) (hv : ci.value? = some v) :
+    TrExpr venv ci.levelParams [] v (.const ci.name (VLevel.params ci.levelParams.length)) := by
+  have {C n ci'} (hC : C.WF) :
+      (SMap.insert C n ci').find? name = some ci →
+      C.find? name = some ci ∨ n = name ∧ ci' = ci := by
+    rw [hC.find?_insert]; simp; split <;> simp +contextual [*]
+  induction H with
+  | empty => simp [SMap.find?] at h
+  | block _ h1 H ih | «axiom» _ _ h1 H ih | «opaque» _ _ h1 H ih =>
+    obtain h | ⟨rfl, rfl⟩ := this H.map_wf h
+    · exact (ih h).mono (VEnv.addConst_le h1)
+    · contradiction
+  | defn h2 h3 h1 H ih =>
+    have' le := (VEnv.addConst_le h1).trans VEnv.addDefEq_le
+    obtain h | ⟨rfl, rfl⟩ := this H.map_wf h
+    · exact (ih h).mono le
+    · cases hv
+      have := VEnv.IsDefEq.extra0 VEnv.addDefEq_self <|
+        (H.defn h2 h3 h1).wf.ordered.defEqWF VEnv.addDefEq_self
+      let ⟨⟨⟨b1, b2, b3⟩, b4⟩, b5⟩ := h2
+      refine ⟨_, b5.mono le, b2.symm ▸ b4.symm ▸ ⟨_, this.symm⟩⟩
+  | quot _ h1 H ih =>
+    suffices ∀ {n k ci' P}, (∀ C env, Aligned safety C env → P C env → C.find? name = some ci) →
+        ∀ C env, Aligned safety C env → AddQuot1 n k ci' P C env → C.find? name = some ci by
+      refine (ih <| this (this <| this <| this ?_) _ _ H.aligned h1).mono h1.le
+      rintro _ _ _ ⟨rfl, rfl⟩; exact h
+    rintro n k ci' P ih C env wf ⟨_, h1, _, h2, h3, h4⟩
+    have wf' := wf.const (.const ⟨by cases safety <;> rfl, h2.2⟩) h3 rfl
+    obtain h | ⟨rfl, rfl⟩ := this wf.map_wf (ih _ _ wf' h4)
+    · exact h
+    · contradiction
+  | induct _ h1 H ih => cases h1
+
+nonrec theorem TrEnv.of_value (H : TrEnv safety env venv) (h : env.find? name = some ci)
+    (hs : isAsSafeAs safety ci) (hv : ci.value? = some v) :
+    TrExpr venv ci.levelParams [] v (.const ci.name (VLevel.params ci.levelParams.length)) :=
+  H.of_value (by rwa [← H.map_wf.find?'_eq_find?]) hs hv
