Lean4Lean/Verify/Typing/Lemmas.lean
@@ -683,6 +683,9 @@ theorem TrExpr.fvarsList (H : TrExpr env Us Δ e e') : e.fvarsList ⊆ Δ.fvars 
 
 theorem TrProj.wf (H1 : TrProj Δ s i e e') (H2 : VExpr.WF env U Γ e) : VExpr.WF env U Γ e' := sorry
 
+theorem TrExpr.wf (H : TrExpr env Us Δ e e') : VExpr.WF env Us.length Δ.toCtx e' :=
+  let ⟨_, _, _, H⟩ := H; ⟨_, H.hasType.2⟩
+
 variable! (henv : Ordered env) {Us : List Name} (hΔ : VLCtx.WF env Us.length Δ) in
 theorem TrExprS.wf (H : TrExprS env Us Δ e e') : VExpr.WF env Us.length Δ.toCtx e' := by
   induction H with
